<?xml version="1.0" encoding="utf-8"?>
<rdf:RDF
  xmlns:rdf="http://www.w3.org/1999/02/22-rdf-syntax-ns#"
  xmlns:rdfs="http://www.w3.org/2000/01/rdf-schema#"
  xmlns:seris="http://forum.eionet.europa.eu/nrc-state-environment/seris/ontology/schema#"
  xmlns:dct="http://purl.org/dc/terms/"
  xmlns:owl="http://www.w3.org/2002/07/owl#"
>
  <owl:Ontology rdf:about="">
    <dct:title>Schema for Seris</dct:title>
    <dct:creator>Iulia Pasov</dct:creator>
    <dct:description>This schema is used for the  State of the Environment Reporting Information System </dct:description>
  </owl:Ontology>

  <!--Classes and Properties-->

  <rdf:Class rdf:ID="SERISReport">
    <rdfs:label xml:lang="en">National state of the environment report
    </rdfs:label>
    <rdfs:comment xml:lang="en">A bibliographic item in the inventory of
    national state of the environment reports (SERIS).
    </rdfs:comment>
    <rdfs:subClassOf rdf:resource="http://purl.org/net/nknouf/ns/bibtex#Entry"/>
    <rdfs:subClassOf rdf:resource="http://uri.gbv.de/ontology/bibo/Document"/>
    <rdfs:subClassOf rdf:resource="http://purl.org/dc/dcmitype/Collection"/>
  </rdf:Class>

  <rdf:Property rdf:ID="structure">
    <rdfs:label xml:lang="en">Structure</rdfs:label>
    <rdfs:comment xml:lang="en">Information about the indicators present in a report's structure</rdfs:comment>
    <rdfs:range rdf:resource="http://www.w3.org/2000/01/rdf-schema#Literal"/>
  </rdf:Property>

  <rdf:Property rdf:ID="hasFocusValue">
    <rdfs:label xml:lang="en">has focus value</rdfs:label>
    <rdfs:comment xml:lang="en">Information about how much the report is focused on several topics. Possible values are: major(chapter), some(sections), minor(ocasionally mentioned), none
    </rdfs:comment>
    <rdfs:range rdf:resource="http://www.w3.org/2000/01/rdf-schema#Literal"/>
  </rdf:Property>

  <rdf:Property rdf:ID="hasIndicatorCount">
    <rdfs:label xml:lang="en">has indicator count</rdfs:label>
    <rdfs:comment xml:lang="en">Information about the number of indicators present in the report. Possible values are: Several(>5), Some(3-5), Few(1-2) or None(0)
    </rdfs:comment>
    <rdfs:range rdf:resource="http://www.w3.org/2000/01/rdf-schema#Literal"/>
  </rdf:Property>

  <rdf:Property rdf:ID="policyRecommendationQuantifier">
    <rdfs:label xml:lang="en">policy recommendation quantifier</rdfs:label>
    <rdfs:comment xml:lang="en">Quentification on whether the report gives policy recommendations. Possible values are: explicitly, implicitly and none.
    </rdfs:comment>
    <rdfs:range rdf:resource="http://www.w3.org/2000/01/rdf-schema#Literal"/>
  </rdf:Property>
</rdf:RDF>
